Test/Interpreter/ub_location.mlir
@@ -1,0 +1,13 @@
+// RUN: veir-interpret %s | filecheck %s
+
+// Check that UB is  reported together with the operation that triggered it.
+"builtin.module"() ({
+  "func.func"() <{sym_name = "main", function_type = () -> i8}> ({
+    %a = "arith.constant"() <{ "value" = 7 : i8 }> : () -> i8
+    %z = "arith.constant"() <{ "value" = 0 : i8 }> : () -> i8
+    %r = "arith.divsi"(%a, %z) : (i8, i8) -> i8
+    "func.return"(%r) : (i8) -> ()
+  }) : () -> ()
+}) : () -> ()
+
+// CHECK: Undefined behavior at: %{{[0-9]+}} = "arith.divsi"
